src/wf.lean
@@ -1,0 +1,53 @@
+-- non-recursive
+inductive simple
+| acon
+| bcon
+
+def f : simple → ℕ
+| simple.acon := 1
+| simple.bcon := 2
+
+#print f
+#print f._main -- uses cases on
+
+inductive recur
+| acon (r : recur)
+| bcon
+
+def g : recur → ℕ
+| (recur.acon r) := g r + 1
+| recur.bcon := 2
+
+#print g
+#print g._main -- uses brec_on (internally uses below)
+#check @recur.cases_on
+#check @recur.brec_on
+
+inductive foo : ℕ → Type
+| acon (n) (r : foo n) : foo (n + 1)
+| bcon : foo 0
+
+def h : Π {n}, foo n → ℕ
+| _ (foo.acon n r) := 
+    have 0 < 0 := sorry,
+    h r
+| n foo.bcon := 0
+using_well_founded {rel_tac := λ_ _, `[exact ⟨_, measure_wf (λ ⟨n, f⟩, 0)⟩]}
+
+#print h
+#print h._main
+#print h._main._pack -- I think the name pack comes from the fact that arguments 
+#print id_rhs
+#reduce id_rhs ℕ 2
+#print h._match_1
+#reduce h._match_1 ⟨0, foo.bcon⟩
+
+inductive bar : ℕ → Type
+| acon (r : bar 1) : bar 0
+| bcon (n) : bar n
+| ccon (n) (l : list (bar 0)) : bar n
+
+def i : Π {n}, bar n → ℕ
+| _ (bar.acon r) := i r
+| _ (bar.bcon n) := 1
+| _ (bar.ccon n l) := 2
